\documentclass{article}
\usepackage[T1]{fontenc}
\usepackage[latin1]{inputenc}
\usepackage[letterpaper]{geometry}
\geometry{verbose, tmargin=2cm, bmargin=2cm, lmargin=2cm, rmargin=2cm}
\setcounter{secnumdepth}{2}
\setcounter{tocdepth}{2}
\usepackage{amstext}
\usepackage{esint}

\makeatother


\author{Daniel Sank}
\title{Fourier Rules}
\date{October 4, 2010}


\begin{document}


\maketitle

\section*{Useful formulae}

\begin{itemize}
\item $\textbf{Trigonometry}$\begin{eqnarray*}
A\cos(x)+B\sin(x) & = & M\cos(x+\phi)\\
\textrm{if}\qquad M^{2}=A^{2}+B^{2} & \textrm{and} & \tan(\phi)=-\frac{B}{A}\end{eqnarray*}
 \begin{eqnarray*}
\cos\left(\alpha+\beta\right) & = & \cos\left(\alpha\right)\cos\left(\beta\right)-\sin\left(\alpha\right)\sin\left(\beta\right)\\
\sin\left(\alpha+\beta\right) & = & \sin\left(\alpha\right)\cos\left(\beta\right)+\cos\left(\alpha\right)\sin\left(\beta\right)\end{eqnarray*}
 \begin{eqnarray*}
\sin\left(\alpha\right)\sin\left(\beta\right) & = & \frac{1}{2}\left[\cos\left(\alpha-\beta\right)-\cos\left(\alpha+\beta\right)\right]\\
\cos\left(\alpha\right)\cos\left(\beta\right) & = & \frac{1}{2}\left[\cos\left(\alpha-\beta\right)+\cos\left(\alpha+\beta\right)\right]\\
\sin\left(\alpha\right)\cos\left(\beta\right) & = & \frac{1}{2}\left[\sin\left(\alpha+\beta\right)+\sin\left(\alpha-\beta\right)\right]\end{eqnarray*}
 \begin{eqnarray*}
\cos\left(x\right)=\sin\left(x+\frac{\pi}{2}\right) & \textrm{and} & \sin\left(x\right)=\cos\left(x-\frac{\pi}{2}\right)\end{eqnarray*}

\end{itemize}

\section*{Fourier transform rules in $t$ and $\nu$}

Checked every line in this section February 2014.

\begin{itemize}
\item \textbf{Fourier transform pair} \begin{eqnarray*}
\tilde{f}(\nu) & = & \int f(t)e^{-i2\pi\nu t}~dt\\
f(t) & = & \int\tilde{f}(\nu)e^{i2\pi\nu t}~d\nu\end{eqnarray*}

\item \textbf{Delta function} \begin{eqnarray*}
\int dt\: e^{i2\pi(\nu-\nu')t} & = & \delta(\nu-\nu')\\
\int d\nu\: e^{i2\pi(t-t')\nu} & = & \delta(t-t')\end{eqnarray*}

\item \textbf{Convolution} \begin{eqnarray*}
\int_{t}f(t)g(t)~e^{-i2\pi Nt}~dt & = & \int_{\nu}\tilde{f}(\nu)\tilde{g}(N-\nu)~d\nu=(\tilde{g}*\tilde{f})(N)\\
\int_{t}(f*g)(t)~e^{-i2\pi\nu t}~dt & = & \tilde{f}(\nu)\tilde{g}(\nu)\\
\int_{\nu}\tilde{f}(\nu)\tilde{g}(\nu)~e^{i2\pi\nu\tau}~d\nu & = & \int_{t}f(t)g(\tau-t)~dt=(f*g)(\tau)\\
\int_{\nu}(\tilde{f}*\tilde{g})(\nu)~e^{i2\pi\nu t}~d\nu & = & f(t)g(t)\end{eqnarray*}

\item $\textbf{Cross Correlation}$\[
\int_{\tau}d\tau e^{-i2\pi N\tau}\left(f\star g\right)(\tau)=\int_{\tau}d\tau e^{-i2\pi N\tau}\left(\int_{t}f(t)^{*}g(t+\tau)dt\right)=\tilde{f}(N)^{*}\tilde{g}(N)\]

\item $\textbf{Weiner Kinchein}$ Consider the cross correlation theorem
with $f=g$. Defining the physicist's power spectrum as $S_{p}(\nu)=\tilde{f}^{*}(\nu)\tilde{f}(\nu)$
we have\begin{eqnarray*}
\int_{\tau}e^{-i2\pi N\tau}(f\star f)(\tau)d\tau & = & \int_{\tau}e^{-i2\pi N\tau}\left(\int_{t}f(t)^{*}f(t+\tau)dt\right)d\tau=\tilde{f}(N)^{*}\tilde{f}(N)=S_{p}(N)\\
\int_{N}S_{p}(N)e^{i2\pi N\tau}dN & = & \int_{t}f(t)^{*}f(t+\tau)\: dt\end{eqnarray*}
\end{itemize}

\subsection*{Real Signals}

Consider $f(t)\in\Re$. Then $\tilde{f}(\nu)^{*}=\tilde{f}(-\nu)$.
Then $S_{p}(N)=\tilde{f}(N)^{*}\tilde{f}(N)=\tilde{f}(-N)\tilde{f}(N)=S_{p}(-N)$.
Therefore we only need to look at positive frequencies to have all
available information about $f$. Define the engineer power spectrum
$S_{e}(N)=2S_{p}(N)$. Then for example we get \begin{eqnarray*}
\int_{\tau}\left(\int_{t}f(t)f(t+\tau)~dt\right)\: e^{-i2\pi N\tau}\: d\tau & = & \frac{1}{2}S_{e}(N)\\
\int_{N=0}^{\infty}S_{e}(N)\:\cos(2\pi N\tau)\: dN & = & \int_{t}f(t)f(t+\tau)\: dt\end{eqnarray*}

\subsection*{Finite Time Series}

Consider a set of experimental data represented by $f(t)$ for $t\in[0,T]$,
ie. we aquire data for a time $T$. Then it makes sense to define
the Fourier transforms as\[
\tilde{f}(\nu)=\frac{1}{\sqrt{T}}\int_{t=0}^{T}f(t)e^{-i2\pi\nu t}dt\]
 We still take\[
S_{p}(\nu)=\tilde{f}(\nu)^{*}\tilde{f}(\nu)\]
 Note that $S_{p}$ now has units of $[f^{2}T]$ or $f^{2}/\textrm{Hz}$.
This is called a $\textbf{power spectral density}$. Now the WK theorem
reads\[
\int_{N=0}^{\infty}S_{e}(N)\:\cos\left(2\pi N\tau\right)\: dN=\frac{1}{T}\int_{t}f(t)f(t+\tau)\: dt\]
 The thing on the right hand side is the autocorrelation function
of $f$. The prefactor normalizes the correlation. Because we now
have this normalization we can replace this autocorrelation with an
$\emph{ensemble}$ average:\[
\frac{1}{T}\int_{t}f(t)f(t+\tau)\: dt=\langle f(0)f(\tau)\rangle\]
 where the equality of these two {}``averages'' is the definition
of an $\textbf{ergodic}$ process, and the enemble average can be
written as $\langle f(0)f(\tau)\rangle$ if we assume the process
is $\textbf{stationary}$. All in all this gives us\begin{eqnarray*}
\int_{N=0}^{\infty}S_{e}(N)\:\cos\left(2\pi N\tau\right)\: dN & = & \langle f(0)f(\tau)\rangle\\
2\int_{-\infty}^{\infty}e^{-i2\pi Nt}\langle f(0)f(t)\rangle dt & = & S_{e}(N)\end{eqnarray*}


\section*{Fourier transform rules in $t$ and $\omega$}

Checked every line February 2014.

\begin{itemize}
\item \textbf{Fourier transform pair} \begin{eqnarray*}
\tilde{f}(\omega) & = & \int f(t)e^{-i\omega t}~dt\\
f(t) & = & \int\tilde{f}(\omega)e^{i\omega t}~\frac{d\omega}{2\pi}\end{eqnarray*}

\item \textbf{Delta function} \begin{eqnarray*}
\int dt~e^{i(\omega-\omega')t} & = & 2\pi\delta(\omega-\omega')\\
\int\frac{d\omega}{2\pi}~e^{i\omega(t-t')} & = & \delta(t-t')\end{eqnarray*}

\item \textbf{Convolution} \begin{eqnarray*}
\int_{t}f(t)g(t)~e^{-i\Omega t}dt & = & \int_{\omega}\tilde{f}(\omega)\tilde{g}(\Omega-\omega)\frac{d\omega}{2\pi}=\frac{1}{2\pi}(\tilde{g}*\tilde{f})(\Omega)\\
\int_{\omega}\tilde{f}(\omega)\tilde{g}(\omega)~e^{i\omega\tau}\frac{d\omega}{2\pi} & = & \int_{t}f(t)g(\tau-t)dt=(f*g)(\tau)\\
\int_{t}(f*g)(t)~e^{-i\omega t}~dt & = & \tilde{f}(\omega)\tilde{g}(\omega)\\
\int_{\omega}(\tilde{f}*\tilde{g})(\omega)~e^{i\omega t}~\frac{d\omega}{2\pi} & = & 2\pi f(t)g(t)\end{eqnarray*}

\item \textbf{Cross Correlation}\begin{equation}
\int d\tau e^{-i\Omega\tau}\left(f\star g\right)(\tau) = \int d\tau e^{-i\Omega\tau}\left(\int f(t)^{*}g(t+\tau)dt\right)=\tilde{f}^{*}(\Omega)\tilde{g}(\Omega) \nonumber \end{equation}

\item \textbf{Weiner Kinchein} Consider the cross correlation theorem in
the case where $g=f$. Defining the physicist power spectrum by $S_{p}^{\infty}(\Omega)=\tilde{f}(\Omega)^{*}\tilde{f}(\Omega)$
we have \begin{eqnarray*}
\int_{\tau}\left(\int_{t}f^{*}(t)f(t+\tau)~dt\right)~e^{-i\Omega\tau}~d\tau & = & S_{p}^{\infty}(\Omega)\\
\int_{\Omega}S_{p}^{\infty}(\Omega)~e^{i\Omega\tau}~\frac{d\Omega}{2\pi} & = & \int_{t}f^{*}(t)f(t+\tau)~dt\end{eqnarray*}
\end{itemize}

\subsection*{Real Signals - $\tilde{f}(\omega)^{*}=\tilde{f}(-\omega)$}
All results in this subsection pertain to real functions of time.

\begin{itemize}

\item $\textbf{Weiner Kinchein:}$ Consider $f(t)\in\Re$. Then $\tilde{f}(\omega)^{*}=\tilde{f}(-\omega)$.
Then $S_{p}^{\infty}(\Omega)=\tilde{f}(\Omega)^{*}\tilde{f}(\Omega)=\tilde{f}(-\Omega)\tilde{f}(-\Omega)^{*}=S_{p}^{\infty}(-\Omega)$.
Therefore we only need to look at positive frequencies to have all
available information about $f$. Define the engineer power spectrum
$S_{e}^{\infty}(\Omega)=2S_{p}^{\infty}(\Omega)$. Then for example
we get \begin{eqnarray*}
\int_{\tau}\left(\int_{t}f(t)f(t+\tau)~dt\right)\: e^{-i\Omega\tau}\: d\tau & = & \frac{1}{2}S_{e}^{\infty}(\Omega)\\
\int_{\Omega=0}^{\infty}S_{e}^{\infty}(\Omega)\:\cos(\Omega\tau)\:\frac{d\Omega}{2\pi} & = & \int_{t}f(t)f(t+\tau)\: dt\\
\textrm{or}\qquad\lim_{T\rightarrow\infty}\frac{1}{T}\int_{\Omega=0}^{\infty}S_{e}^{T}(\Omega)\cos(\Omega\tau)\,\frac{d\Omega}{2\pi} & = & \lim_{T\rightarrow\infty}\frac{1}{T}\int_{-T/2}^{T/2}f(t)f(t+\tau)\, dt\end{eqnarray*}

\item $\textbf{Sine/Cosine Representation}$
For real functions $f$ there is a particularly useful decomposition into sine and cosine functions.
\begin{eqnarray*}
f(t) & = & \int\frac{d\omega}{2\pi}\tilde{f}(\omega)e^{i\omega t}\\
 & = & \int_{0}^{\infty}\frac{d\omega}{2\pi}\left[e^{i\omega t}\tilde{f}(\omega)+e^{-i\omega t}\tilde{f}(\omega)^{*}\right]\\
 & = & \int_{0}^{\infty}\frac{d\omega}{2\pi}\cos(\omega t)\left[\tilde{f}(\omega)^{*}+\tilde{f}(\omega)\right]+i\sin(\omega t)\left[\tilde{f}(\omega)-\tilde{f}(\omega)^{*}\right]\\
 & = & 2 \int_{0}^{\infty}\frac{d\omega}{2\pi}\left[\Re\tilde{f}(\omega)\cos(\omega t)-\Im\tilde{f}(\omega)\sin(\omega t)\right]\end{eqnarray*}
 or alternately\[
f(t)= 2 \int_{0}^{\infty}\frac{d\omega}{2\pi}\sqrt{S_{p}(\omega)}\cos\left(\omega t+\phi(\omega)\right)\]
 where\[
S_{p}(\omega)=\Re\tilde{f}(\omega)^{2}+\Im\tilde{f}(\omega)^{2}=|\tilde{f}(\omega)|^{2}\qquad\textrm{and}\qquad\tan\left(\phi(\omega)\right)=\frac{\Im\tilde{f}}{\Re\tilde{f}}\]

\item $\textbf{Weiner Kinchein revisit:}$ Consider a set of experimental data
represented by $f(t)$ for $t\in[0,T]$, ie. we aquire data for a
time $T$. Then it makes sense to define the Fourier transforms as\[
\tilde{f}(\omega)=\frac{1}{\sqrt{T}}\int_{t=0}^{T}f(t)e^{-i\omega t}dt\]
 We still take\[
S_{p}(\omega)=\tilde{f}(\omega)^{*}\tilde{f}(\omega)\]
 Note that $S_{p}$ now has units of $[f^{2}T]$ or $f^{2}/\textrm{Hz}$.
This is called a $\textbf{power spectral density}$. Now the WK theorem
reads\[
\int_{\Omega=0}^{\infty}S_{e}(\Omega)\:\cos\left(\Omega\tau\right)\:\frac{d\Omega}{2\pi}=\frac{1}{T}\int_{t}f(t)f(t+\tau)\: dt\]
 The thing on the right hand side is the autocorrelation function
of $f$. The prefactor normalizes the correlation. Because we now
have this normalization we can replace this autocorrelation with an
$\emph{ensemble}$ average:\[
\frac{1}{T}\int_{t}f(t)f(t+\tau)\: dt=\langle f(0)f(\tau)\rangle\]
 where the equality of these two {}``averages'' is the definition
of an $\textbf{ergodic}$ process, and the enemble average can be
written as $\langle f(0)f(\tau)\rangle$ if we assume the process
is $\textbf{stationary}$. All in all this gives us\[
\int_{\Omega=0}^{\infty}S_{e}(\Omega)\:\cos\left(\Omega\tau\right)\:\frac{d\Omega}{2\pi}=\langle f(0)f(\tau)\rangle\]

\end{itemize}

\section{Delta functions}

\begin{equation}
\int T \frac{\sin \left( \omega T / 2 \right)}{\left( \omega T / 2 \right)} \frac{d\omega}{2\pi} = 1 \end{equation}

\end{document}
