\levelstay{Uniform Linear Transformation}

\leveldown{Problem}

Prove $U(\alpha, \beta) = \alpha + \beta U(0, 1)$ by showing that
\begin{equation*}
  M_{U(\alpha, \beta)}(t) = M_{\alpha + \beta U(0, 1)}(t) \, .
\end{equation*}
Note: $U(\alpha, \beta)$ is a uniform distribution with mean $\alpha$ and width $\beta$.

\levelstay{Solution}

The characteristic function $M_{U(0, 1)}(t)$ is
\begin{equation*}
  M_{U(0, 1)}(t) = \int_{-1/2}^{1/2} e^{xt} \, dt = i \frac{\sin(t/2)}{t/2} \, .
\end{equation*}

Let us find $M_{U(0, \beta)}$.
Consider a random variable $X$ and another random variable $Y$ defined by $y = Ax$.
Using the change of variables theorem, we can show that $M_{AX}(t) = M_X(At)$.
Therefore, we have
\begin{equation*}
  M_{\beta U(0, 1)}(t) = M_{U(0, 1)}(\beta t) = i \frac{\sin(\beta t / 2)}{\beta t / 2} \, .
\end{equation*}

Now consider $M_{U(\alpha, \beta)}(t)$.
The effect of the $\alpha$ is to shift the distribution by $\alpha$ to the right.
We can represent this by considering random variables $X$ and $Y$ related by $y = x + \alpha$.
Then
\begin{equation*}
  M_Y(t)
  =              \int P_Y(y) e^{yt} \, dy \\
  =              \int P_X(y - \alpha) e^{yt} \, dy \\
  =              \int P_X(x) e^{(x + \alpha)t} \, dx \\
  = e^{\alpha t} M_X(t) \, .
\end{equation*}
Therefore,
\begin{equation*}
  M_{\alpha + \beta U(0, 1)}(t)
  = e^{\alpha t} M_{\beta U(0, 1)}(t)
  = e^{\alpha t} i \frac{\sin(\beta t/2)}{\beta t/2}\, ,
\end{equation*}
which matches the form of $M_{U(\alpha, \beta)}(t)$ that we can compute using direct integration.
